fix: private lemmas

Std/Data/ByteArray.lean
@@ -4,7 +4,6 @@ Released under Apache 2.0 license as described in the file LICENSE.
 Authors: François G. Dorais
 -/
 import Std.Data.Array.Lemmas
-import Std.Data.Fin.Basic
 import Std.Tactic.Ext.Attr
 
 namespace ByteArray
@@ -23,6 +22,8 @@ theorem getElem_eq_data_getElem (a : ByteArray) (h : i < a.size) : a[i] = a.data
     a.uset i v h = a.set ⟨i.toNat, h⟩ v := rfl
 
 /-! ### empty -/
+
+@[simp] theorem mkEmpty_data (cap) : (mkEmpty cap).data = #[] := rfl
 
 @[simp] theorem empty_data : empty.data = #[] := rfl
 
@@ -129,16 +130,15 @@ def ofFn (f : Fin n → UInt8) : ByteArray where
 @[simp] theorem getElem_ofFn (f : Fin n → UInt8) (i) (h : i < (ofFn f).size):
     (ofFn f)[i] = f ⟨i, size_ofFn f ▸ h⟩ := get_ofFn ..
 
-/-- More efficient implementation of `ByteArray.ofFn` -/
-def ofFnAux (f : Fin n → UInt8) : ByteArray := go 0 (mkEmpty n) where
-  /-- Auxiliary for `ofFnAux` -/
+private def ofFnAux (f : Fin n → UInt8) : ByteArray := go 0 (mkEmpty n) where
   go (i : Nat) (acc : ByteArray) : ByteArray :=
     if h : i < n then go (i+1) (acc.push (f ⟨i, h⟩)) else acc
 termination_by _ => n - i
 
+private theorem ofFnAux_data (f : Fin n → UInt8) :
+    (ofFnAux.go f i acc).data = Array.ofFn.go f i acc.data := by
+  rw [ofFnAux.go, Array.ofFn.go]; split; rw [ofFnAux_data, push_data]; rfl
+termination_by _ => n - i
+
 @[csimp] theorem ofFn_eq_ofFnAux : @ofFn = @ofFnAux := by
-  let rec ofFnAux_data (f : Fin n → UInt8) :
-      (ofFnAux.go f i acc).data = Array.ofFn.go f i acc.data := by
-    rw [ofFnAux.go, Array.ofFn.go]; split; rw [ofFnAux_data, push_data]; rfl
-  termination_by _ => n - i
-  funext n f; ext; simp [ofFnAux, Array.ofFn, ofFnAux_data, mkEmpty]
+  funext n f; ext; simp [ofFnAux, ofFnAux_data, Array.ofFn]
